put wip

pulse/ulib/experimental/Steel.Hashtbl.fst
@@ -48,6 +48,9 @@ assume val bv_unset (#n:U32.t) (i:U32.t{U32.v i < U32.v n}) (bv:bv_t n)
          (requires True)
          (ensures fun r -> (~ (bv_is_set i r)) /\
                         (forall (j:U32.t{U32.v j < U32.v n}). j =!= i ==> bv_is_set j r == bv_is_set j bv))
+assume val bv_init (n:U32.t) : bv_t n
+assume val bv_init_all_unset (n:U32.t)
+  : Lemma (forall (i:U32.t{U32.v i < U32.v n}). ~ (bv_is_set i (bv_init n)))
 
 noeq
 type tbl #k #v #contents (#vp:vp_t k v contents) (h:hash_fn k) (finalizer:finalizer_t vp) = {
@@ -86,17 +89,6 @@ let store_and_repr_related
       | None -> True
       | Some (k, _) -> Map.contains k m
 
-// let store_and_borrows_related
-//   (#k:eqtype)
-//   (#v:Type0)
-//   (s:Seq.seq (option (k & v)))
-//   (borrows:Map.t k v)
-//   : prop
-//   = forall (x:k). Map.contains x borrows ==>
-//              (exists (i:nat{i < Seq.length s}) (y:v).
-//                 Seq.index s i == Some (x, y) /\
-//                 Map.sel x borrows == Some y)
-
 let store_and_bv_and_borrows_related
   (#k:eqtype)
   (#v:Type0)
@@ -112,6 +104,31 @@ let store_and_bv_and_borrows_related
         if bv_is_set (U32.uint_to_t i) bv
         then Map.sel x borrows == Some y
         else ~ (Map.contains x borrows)
+
+let store_and_borrows_related
+  (#k:eqtype)
+  (#v:Type0)
+  (#n:U32.t)
+  (bv:bv_t n)
+  (s:Seq.seq (option (k & v)))
+  (borrows:Map.t k v)
+  : Lemma (requires store_and_bv_and_borrows_related bv s borrows)
+          (ensures forall (x:k). Map.contains x borrows ==>
+                            (exists (i:nat{i < Seq.length s}) (y:v).
+                            Seq.index s i == Some (x, y) /\
+                            Map.sel x borrows == Some y))
+  = admit ()
+
+// let test_store_and_borrows_related
+//   (#k:eqtype)
+//   (#v:Type0)
+//   (#n:U32.t)
+//   (bv:bv_t n)
+//   (s:Seq.seq (option (k & v)))
+//   (borrows:Map.t k v)
+//   : Lemma (requires store_and_bv_and_borrows_related bv s borrows)
+//           (ensures store_and_borrows_related s borrows)
+//   = ()
 
 module CE = FStar.Algebra.CommMonoid.Equiv
 module SeqPerm = FStar.Seq.Permutation
@@ -160,6 +177,46 @@ let value_vprops
   : vprop
   = SeqPerm.foldm_snoc vprop_monoid (value_vprops_seq vp s m borrows)
 
+let pure_invariant
+  (#k:eqtype)
+  (#v #contents:Type0)
+  (#vp:vp_t k v contents)
+  (#h:hash_fn k)
+  (#finalizer:finalizer_t vp)
+  (arr:tbl h finalizer)
+  (m:repr k contents)
+  (borrows:Map.t k v)
+  (bv:bv_t arr.store_len)
+  (s:Seq.seq (option (k & v)))
+  : prop
+  = seq_props h s /\
+    store_and_repr_related s m /\
+    store_and_bv_and_borrows_related bv s borrows
+
+
+[@@__reduce__]
+let store_contents_pred_seq
+  (#k:eqtype)
+  (#v #contents:Type0)
+  (#vp:vp_t k v contents)
+  (#h:hash_fn k)
+  (#finalizer:finalizer_t vp)
+  (arr:tbl h finalizer)
+  (m:repr k contents)
+  (borrows:Map.t k v)
+  (bv:bv_t arr.store_len)
+  : Seq.seq (option (k & v)) -> vprop
+  = fun s ->
+    A.pts_to arr.store s
+      `star`
+    GR.pts_to arr.g_repr full_perm m
+      `star`
+    GR.pts_to arr.g_borrows full_perm borrows
+      `star`
+    pure (pure_invariant arr m borrows bv s)
+      `star`
+    value_vprops vp s m borrows
+
 [@@__reduce__]
 let store_contents_pred
   (#k:eqtype)
@@ -170,23 +227,14 @@ let store_contents_pred
   (arr:tbl h finalizer)
   (m:repr k contents)
   (borrows:Map.t k v)
-  : Seq.seq (option (k & v)) -> vprop
-  = fun s ->
-    A.pts_to arr.store s
+  : bv_t arr.store_len -> vprop
+  = fun bv ->
+    R.pts_to arr.bv_borrows full_perm bv
       `star`
-    GR.pts_to arr.g_repr full_perm m
-      `star`
-    GR.pts_to arr.g_borrows full_perm borrows
-      `star`
-    pure (seq_props h s /\
-          store_and_repr_related s m /\
-          store_and_borrows_related s borrows)
-      `star`
-    value_vprops vp s m borrows
+    exists_ (store_contents_pred_seq arr m borrows bv)
 
 [@@__reduce__]
 let tperm arr m borrows = exists_ (store_contents_pred arr m borrows)
-
 
 assume val admit__ (#opened:_) (#a:Type) (#p:pre_t) (#q:post_t a) (_:unit)
   : STAtomicF a opened p q True (fun _ -> False)
@@ -200,36 +248,52 @@ assume val rewrite_equiv (#opened:_) (p q:vprop)
 
 let create #k #v #contents #vp h finalizer n =
   let store = A.alloc #(option (k & v)) None n in
+  let bv_borrows = R.alloc (bv_init n) in
   let g_repr = GR.alloc (G.hide (Map.empty k contents)) in
   let g_borrows = GR.alloc (G.hide (Map.empty k v)) in
   let arr : tbl #k #v #contents #vp h finalizer = {
     store_len = n;
     store = store;
+    bv_borrows = bv_borrows;
     g_repr = g_repr;
     g_borrows = g_borrows;
     store_len_pf = () } in
+  
   rewrite (A.pts_to store (Seq.create #(option (k & v)) (U32.v n) None)
+             `star`
+           R.pts_to bv_borrows full_perm (bv_init n)
              `star`
            GR.pts_to g_repr full_perm (Map.empty k contents)
              `star`
            GR.pts_to g_borrows full_perm (Map.empty k v))
           (A.pts_to arr.store (Seq.create #(option (k & v)) (U32.v n) None)
              `star`
+           R.pts_to arr.bv_borrows full_perm (bv_init arr.store_len)
+             `star`
            GR.pts_to arr.g_repr full_perm (Map.empty k contents)
              `star`
            GR.pts_to arr.g_borrows full_perm (Map.empty k v));
+
   foldm_snoc_unit_seq
     vprop_monoid
-    (value_vprops_seq vp (Seq.create #(option (k & v)) (U32.v n) None)
+    (value_vprops_seq vp (Seq.create (U32.v n) None)
                          (Map.empty k contents)
                          (Map.empty k v));
-  rewrite_equiv emp (value_vprops vp (Seq.create #(option (k & v)) (U32.v n) None)
+  rewrite_equiv emp (value_vprops vp (Seq.create (U32.v n) None)
                                      (Map.empty k contents)
                                      (Map.empty k v));
-  intro_pure (seq_props h (Seq.create #(option (k & v)) (U32.v n) None) /\
-              store_and_repr_related (Seq.create #(option (k & v)) (U32.v n) None) (Map.empty k contents) /\
-              store_and_borrows_related (Seq.create #(option (k & v)) (U32.v n) None) (Map.empty k v));  
-  intro_exists (Seq.create #(option (k & v)) (U32.v n) None)
+
+  bv_init_all_unset arr.store_len;
+  intro_pure (pure_invariant
+    arr
+    (Map.empty k contents)
+    (Map.empty k v)
+    (bv_init arr.store_len)
+    (Seq.create (U32.v n) None));
+  
+  intro_exists (Seq.create (U32.v n) None)
+               (store_contents_pred_seq arr (Map.empty k contents) (Map.empty k v) (bv_init arr.store_len));
+  intro_exists (bv_init arr.store_len)
                (store_contents_pred arr (Map.empty k contents) (Map.empty k v));
   return arr
 
@@ -251,170 +315,47 @@ let value_vprop_seq_upd_borrows
   : Lemma (requires Some? (Seq.index s idx) /\
                     seq_props h s)
           (ensures (let Some (i, x) = Seq.index s idx in
-                    let s0 = value_vprops_seq vp s m borrows in
-                    let s1 = value_vprops_seq vp s m (Map.upd i x borrows) in
-                    Seq.equal (Seq.slice s0 0 idx)
-                              (Seq.slice s1 0 idx) /\
-                    Seq.equal (Seq.slice s0 (idx+1) (Seq.length s))
-                              (Seq.slice s1 (idx+1) (Seq.length s))))
-  = ()
+                    let upd_borrows = Map.upd i x borrows in
+                    value_vprops vp (Seq.slice s 0 idx) m borrows ==
+                    value_vprops vp (Seq.slice s 0 idx) m upd_borrows /\
+                    value_vprops vp (Seq.slice s (idx+1) (Seq.length s)) m borrows ==
+                    value_vprops vp (Seq.slice s (idx+1) (Seq.length s)) m upd_borrows))
+  = let Some (i, x) = Seq.index s idx in
+    let upd_borrows = Map.upd i x borrows in
+    assert (Seq.equal (value_vprops_seq vp (Seq.slice s 0 idx) m borrows)
+                      (value_vprops_seq vp (Seq.slice s 0 idx) m upd_borrows));
+    assert (Seq.equal (value_vprops_seq vp (Seq.slice s (idx+1) (Seq.length s)) m borrows)
+                      (value_vprops_seq vp (Seq.slice s (idx+1) (Seq.length s)) m upd_borrows))
 
-let seq_split3 (#a:Type) (s:Seq.seq a) (i:nat{i < Seq.length s})
-  : (s':(Seq.seq a & Seq.seq a & Seq.seq a){
-     let s1, s2, s3 = s' in
-     Seq.equal s (Seq.append s1 (Seq.append s2 s3))})
-  = Seq.slice s 0 i,
-    Seq.create 1 (Seq.index s i),
-    Seq.slice s (i+1) (Seq.length s)
+let value_vprop_seq_upd_seq_and_repr
+  (#k:eqtype)
+  (#v #contents:Type0)
+  (h:hash_fn k)
+  (vp:vp_t k v contents)
+  (s:Seq.seq (option (k & v)))
+  (m:repr k contents)
+  (borrows:Map.t k v)
+  (idx:nat{idx < Seq.length s})
+  (x:k) (y:v) (c:G.erased contents)
+  : Lemma (requires None? (Seq.index s idx) /\
+                    seq_props h s /\
+                    seq_props h (Seq.upd s idx (Some (x, y))) /\
+                    store_and_repr_related s m)
+          (ensures (let s1 = Seq.upd s idx (Some (x, y)) in
+                    let m1 = Map.upd x (G.reveal c) m in
+                    value_vprops vp (Seq.slice s 0 idx) m borrows ==
+                    value_vprops vp (Seq.slice s1 0 idx) m1 borrows /\
+                    value_vprops vp (Seq.slice s (idx+1) (Seq.length s)) m borrows ==
+                    value_vprops vp (Seq.slice s1 (idx+1) (Seq.length s1)) m1 borrows))
+  = let s1 = Seq.upd s idx (Some (x, y)) in
+    let m1 = Map.upd x (G.reveal c) m in
+    assert (Seq.index s1 idx == Some (x, y));
+    assert (Seq.equal (value_vprops_seq vp (Seq.slice s 0 idx) m borrows)
+                      (value_vprops_seq vp (Seq.slice s1 0 idx) m1 borrows));
+    assert (Seq.equal (value_vprops_seq vp (Seq.slice s (idx+1) (Seq.length s)) m borrows)
+                      (value_vprops_seq vp (Seq.slice s1 (idx+1) (Seq.length s1)) m1 borrows))
 
-let foldm_snoc_split3 (s s1 s2 s3:Seq.seq vprop)
-  : Lemma (requires Seq.equal s (Seq.append s1 (Seq.append s2 s3)))
-          (ensures SeqPerm.foldm_snoc vprop_monoid s
-                     `equiv`
-                   (SeqPerm.foldm_snoc vprop_monoid s1
-                      `star`
-                    (SeqPerm.foldm_snoc vprop_monoid s2
-                       `star`
-                     SeqPerm.foldm_snoc vprop_monoid s3)))
-  = SeqPerm.foldm_snoc_append vprop_monoid s1 (Seq.append s2 s3);
-    SeqPerm.foldm_snoc_append vprop_monoid s2 s3;
-    star_equiv (SeqPerm.foldm_snoc vprop_monoid s1)
-               (SeqPerm.foldm_snoc vprop_monoid (Seq.append s2 s3))
-               (SeqPerm.foldm_snoc vprop_monoid s2
-                  `star`
-                SeqPerm.foldm_snoc vprop_monoid s3);
-    equiv_trans (SeqPerm.foldm_snoc vprop_monoid s)
-                (SeqPerm.foldm_snoc vprop_monoid s1
-                   `star`
-                 (SeqPerm.foldm_snoc vprop_monoid (Seq.append s2 s3)))
-                (SeqPerm.foldm_snoc vprop_monoid s1
-                   `star`
-                 (SeqPerm.foldm_snoc vprop_monoid s2
-                    `star`
-                  SeqPerm.foldm_snoc vprop_monoid s3))
-
-let equiv_helper_q_emp (p q r:vprop)
-  : Lemma (requires q `equiv` emp)
-          (ensures (p `star` (q `star` r)) `equiv` (p `star` r))
-  = equiv_refl r;
-    star_congruence q r emp r;
-    equiv_refl p;
-    star_congruence p (q `star` r) p (emp `star` r);
-    cm_identity r;
-    star_congruence p (emp `star` r) p r;
-    equiv_trans (p `star` (q `star` r))
-                (p `star` (emp `star` r))
-                (p `star` r)
-
-#push-options "--warn_error -271"
-let get #k #v #contents #vp #h #finalizer #m #borrows a i =
-  let equiv_trans (p q r:vprop)
-    : Lemma (requires p `equiv` q /\ q `equiv` r)
-            (ensures p `equiv` r)
-            [SMTPat ()]
-    = equiv_trans p q r in
-  let s = elim_exists () in  
-  elim_pure (seq_props h s /\
-             store_and_repr_related s m /\
-             store_and_borrows_related s borrows);
-  A.pts_to_length a.store s;
-  let idx = h i `U32.rem` a.store_len in
-  let vopt = A.read a.store idx in
-  let r = match vopt with
-          | None -> Absent
-          | Some (i', x) ->
-            if i <> i' then Missing i'
-            else Present x in
-  (match vopt returns STGhostT unit Set.empty _ (fun _ -> get_post m borrows a i r) with
-   | None ->
-     intro_pure (seq_props h s /\
-                 store_and_repr_related s m /\
-                 store_and_borrows_related s borrows);
-     intro_exists (G.reveal s) (store_contents_pred a m borrows);
-     rewrite (tperm a m borrows) (get_post m borrows a i r)
-   | Some (i', x) ->
-     if i <> i'
-     then begin
-       intro_pure (map_contains_prop i' m);
-       intro_pure (seq_props h s /\
-                   store_and_repr_related s m /\
-                   store_and_borrows_related s borrows);
-       intro_exists (G.reveal s) (store_contents_pred a m borrows);
-       rewrite (tperm a m borrows
-                  `star`
-                pure (map_contains_prop i' m))
-               (get_post m borrows a i r)
-     end
-     else begin
-       let vs0 = value_vprops_seq vp s m borrows in
-       let vs0_prefix, vs0_idx, vs0_suffix = seq_split3 vs0 (U32.v idx) in
-       foldm_snoc_split3 vs0 vs0_prefix vs0_idx vs0_suffix;
-       rewrite_equiv (SeqPerm.foldm_snoc vprop_monoid (value_vprops_seq vp s m borrows))
-                     (SeqPerm.foldm_snoc vprop_monoid vs0_prefix
-                        `star`
-                      (SeqPerm.foldm_snoc vprop_monoid vs0_idx
-                         `star`
-                       SeqPerm.foldm_snoc vprop_monoid vs0_suffix));
-
-       let upd_borrows = Map.upd i x borrows in
-
-       let vs1 = value_vprops_seq vp s m upd_borrows in
-       let vs1_prefix, vs1_idx, vs1_suffix = seq_split3 vs1 (U32.v idx) in
-  
-       calc (equiv) {
-         value_vprops vp s m upd_borrows;
-         (equiv) { foldm_snoc_split3 vs1 vs1_prefix vs1_idx vs1_suffix }
-         SeqPerm.foldm_snoc vprop_monoid vs1_prefix
-           `star`
-         (SeqPerm.foldm_snoc vprop_monoid vs1_idx
-            `star`
-          SeqPerm.foldm_snoc vprop_monoid vs1_suffix);
-         (equiv) { value_vprop_seq_upd_borrows h vp s m borrows (U32.v idx);
-                   Classical.forall_intro equiv_refl }
-         SeqPerm.foldm_snoc vprop_monoid vs0_prefix
-           `star`
-         (SeqPerm.foldm_snoc vprop_monoid vs1_idx
-            `star`
-          SeqPerm.foldm_snoc vprop_monoid vs0_suffix);
-         (equiv) { assert (Seq.index vs1 (U32.v idx) == emp);
-                   SeqPerm.foldm_snoc_singleton vprop_monoid emp;
-                   equiv_helper_q_emp (SeqPerm.foldm_snoc vprop_monoid vs0_prefix)
-                                      (SeqPerm.foldm_snoc vprop_monoid vs1_idx)
-                                      (SeqPerm.foldm_snoc vprop_monoid vs0_suffix) }
-         SeqPerm.foldm_snoc vprop_monoid vs0_prefix
-           `star`
-         SeqPerm.foldm_snoc vprop_monoid vs0_suffix;
-       };
-       equiv_sym (value_vprops vp s m upd_borrows)
-                 (SeqPerm.foldm_snoc vprop_monoid vs0_prefix
-                    `star`
-                  SeqPerm.foldm_snoc vprop_monoid vs0_suffix);
-       rewrite_equiv (SeqPerm.foldm_snoc vprop_monoid vs0_prefix
-                          `star`
-                      SeqPerm.foldm_snoc vprop_monoid vs0_suffix)
-                     (value_vprops vp s m (Map.upd i x borrows));
-       let Some c = Map.sel i m in
-       assert (Seq.index vs0 (U32.v idx) == vp i x c);
-       SeqPerm.foldm_snoc_singleton vprop_monoid (vp i x c);
-       assert (equiv (SeqPerm.foldm_snoc vprop_monoid vs0_idx) (vp i x c));
-       rewrite_equiv (SeqPerm.foldm_snoc vprop_monoid vs0_idx) (vp i x c);
-       GR.write a.g_borrows (Map.upd i x borrows);
-       intro_pure (seq_props h s /\
-                   store_and_repr_related s m /\
-                   store_and_borrows_related s (Map.upd i x borrows));
-       intro_exists (G.reveal s) (store_contents_pred a m (Map.upd i x borrows));
-       rewrite (tperm a m (Map.upd i x borrows)
-                  `star`
-                vp i x c)
-               (get_post m borrows a i r)
-     end);
-
-  return r
-#pop-options
-
-let put #k #v #contents #vp #h #finalizer #m #borrows a i x c = admit__ ()
-
-assume val value_vprops_split3
+let value_vprops_split3
   (#k:eqtype)
   (#v #contents:Type0)
   (vp:vp_t k v contents)
@@ -432,6 +373,200 @@ assume val value_vprops_split3
             value_vprops vp s2 m borrows
               `star`
             value_vprops vp s3 m borrows))
+  = admit ()
+
+// let seq_split3 (#a:Type) (s:Seq.seq a) (i:nat{i < Seq.length s})
+//   : (s':(Seq.seq a & Seq.seq a & Seq.seq a){
+//      let s1, s2, s3 = s' in
+//      Seq.equal s (Seq.append s1 (Seq.append s2 s3))})
+//   = Seq.slice s 0 i,
+//     Seq.create 1 (Seq.index s i),
+//     Seq.slice s (i+1) (Seq.length s)
+
+// let foldm_snoc_split3 (s s1 s2 s3:Seq.seq vprop)
+//   : Lemma (requires Seq.equal s (Seq.append s1 (Seq.append s2 s3)))
+//           (ensures SeqPerm.foldm_snoc vprop_monoid s
+//                      `equiv`
+//                    (SeqPerm.foldm_snoc vprop_monoid s1
+//                       `star`
+//                     (SeqPerm.foldm_snoc vprop_monoid s2
+//                        `star`
+//                      SeqPerm.foldm_snoc vprop_monoid s3)))
+//   = 
+
+// let equiv_helper_q_emp (p q r:vprop)
+//   : Lemma (requires q `equiv` emp)
+//           (ensures (p `star` (q `star` r)) `equiv` (p `star` r))
+//   = equiv_refl r;
+//     star_congruence q r emp r;
+//     equiv_refl p;
+//     star_congruence p (q `star` r) p (emp `star` r);
+//     cm_identity r;
+//     star_congruence p (emp `star` r) p r;
+//     equiv_trans (p `star` (q `star` r))
+//                 (p `star` (emp `star` r))
+//                 (p `star` r)
+
+#push-options "--ifuel 2 --fuel 0 --z3rlimit_factor 2"
+let get #k #v #contents #vp #h #finalizer #m #borrows a i =
+  let bv = elim_exists () in
+  let s = elim_exists () in
+  elim_pure (pure_invariant a m borrows bv s);
+  A.pts_to_length a.store s;
+  let idx = h i `U32.rem` a.store_len in
+  let vopt = A.read a.store idx in
+  let r = match vopt with
+          | None -> Absent
+          | Some (i', x) ->
+            if i <> i' then Missing i'
+            else Present x in
+  (match vopt returns STT unit _ (fun _ -> get_post m borrows a i r) with
+   | None ->
+     intro_pure (pure_invariant a m borrows bv s);
+     intro_exists (G.reveal s) (store_contents_pred_seq a m borrows bv);
+     intro_exists (G.reveal bv) (store_contents_pred a m borrows);
+     rewrite (tperm a m borrows) (get_post m borrows a i r)
+   | Some (i', x) ->
+     if i <> i'
+     then begin
+       intro_pure (map_contains_prop i' m);
+       intro_pure (pure_invariant a m borrows bv s);
+       intro_exists (G.reveal s) (store_contents_pred_seq a m borrows bv);
+       intro_exists (G.reveal bv) (store_contents_pred a m borrows);
+       rewrite (tperm a m borrows
+                  `star`
+                pure (map_contains_prop i' m))
+               (get_post m borrows a i r)
+     end
+     else begin
+       value_vprops_split3 vp s m borrows (U32.v idx);
+       rewrite_equiv (value_vprops vp s m borrows)
+                     (value_vprops vp (Seq.slice s 0 (U32.v idx)) m borrows
+                        `star`
+                      value_vprops vp (Seq.create 1 (Seq.index s (U32.v idx))) m borrows
+                        `star`
+                      value_vprops vp (Seq.slice s (U32.v idx+1) (Seq.length s)) m borrows);
+       
+       SeqPerm.foldm_snoc_singleton vprop_monoid (vp i x (Some?.v (Map.sel i m)));
+       assert (Seq.index (value_vprops_seq vp s m borrows) (U32.v idx) == vp i x (Some?.v (Map.sel i m)));
+       assert (Seq.equal (value_vprops_seq vp (Seq.create 1 (Seq.index s (U32.v idx))) m borrows)
+                         (Seq.create 1 (vp i x (Some?.v (Map.sel i m)))));
+       rewrite_equiv (value_vprops vp (Seq.create 1 (Seq.index s (U32.v idx))) m borrows) (vp i x (Some?.v (Map.sel i m)));
+
+       value_vprop_seq_upd_borrows h vp s m borrows (U32.v idx);
+ 
+       rewrite (value_vprops vp (Seq.slice s 0 (U32.v idx)) m borrows
+                  `star`
+                value_vprops vp (Seq.slice s (U32.v idx+1) (Seq.length s)) m borrows)
+               (value_vprops vp (Seq.slice s 0 (U32.v idx)) m (Map.upd i x borrows)
+                  `star`
+                value_vprops vp (Seq.slice s (U32.v idx+1) (Seq.length s)) m (Map.upd i x borrows));
+
+       SeqPerm.foldm_snoc_singleton vprop_monoid emp;
+       assert (Seq.index (value_vprops_seq vp s m (Map.upd i x borrows)) (U32.v idx) == emp);
+       assert (Seq.equal (value_vprops_seq vp (Seq.create 1 (Seq.index s (U32.v idx))) m (Map.upd i x borrows))
+                         (Seq.create 1 emp));
+       rewrite_equiv emp (value_vprops vp (Seq.create 1 (Seq.index s (U32.v idx))) m (Map.upd i x borrows));
+
+       value_vprops_split3 vp s m (Map.upd i x borrows) (U32.v idx);
+       rewrite_equiv
+         (value_vprops vp (Seq.slice s 0 (U32.v idx)) m (Map.upd i x borrows)
+            `star`
+          value_vprops vp (Seq.create 1 (Seq.index s (U32.v idx))) m (Map.upd i x borrows)
+            `star`
+          value_vprops vp (Seq.slice s (U32.v idx+1) (Seq.length s)) m (Map.upd i x borrows))
+         (value_vprops vp s m (Map.upd i x borrows));
+
+       let bv : bv_t a.store_len = R.read a.bv_borrows in
+       R.write a.bv_borrows (bv_set idx bv);
+
+       GR.write a.g_borrows (Map.upd i x borrows);
+
+       intro_pure (pure_invariant a m (Map.upd i x borrows) (bv_set idx bv) s);
+       intro_exists (G.reveal s) (store_contents_pred_seq a m (Map.upd i x borrows) (bv_set idx bv));
+       intro_exists (bv_set idx bv) (store_contents_pred a m (Map.upd i x borrows));
+       rewrite (tperm a m (Map.upd i x borrows)
+                 `star`
+                vp i x (Some?.v (Map.sel i m)))
+               (get_post m borrows a i r)
+     end);
+     return r
+
+let put #k #v #contents #vp #h #finalizer #m #borrows a i x c =
+  let bv = elim_exists () in
+  let s = elim_exists () in
+  elim_pure (pure_invariant a m borrows bv s);
+  A.pts_to_length a.store s;
+  let idx = h i `U32.rem` a.store_len in
+  let vopt = A.read a.store idx in
+  let bv = R.read a.bv_borrows in
+  let r = match vopt with
+          | None -> Put_success
+          | Some (i', x') ->
+            if bv_is_set idx bv
+            then Put_collision_borrowed i' x' (Some?.v (Map.sel i' m))
+            else Put_success in
+  (match vopt returns STT unit _ (fun _ -> put_post m borrows a i x c r) with
+   | None ->
+     A.write a.store idx (Some (i, x));
+     GR.write a.g_repr (Map.upd i (G.reveal c) m);
+     value_vprops_split3 vp s m borrows (U32.v idx);
+     rewrite_equiv (value_vprops vp s m borrows)
+                   (value_vprops vp (Seq.slice s 0 (U32.v idx)) m borrows
+                      `star`
+                    value_vprops vp (Seq.create 1 (Seq.index s (U32.v idx))) m borrows
+                      `star`
+                    value_vprops vp (Seq.slice s (U32.v idx+1) (Seq.length s)) m borrows);
+     SeqPerm.foldm_snoc_singleton vprop_monoid emp;
+     assert (Seq.index (value_vprops_seq vp s m borrows) (U32.v idx) == emp);
+     assert (Seq.equal (value_vprops_seq vp (Seq.create 1 (Seq.index s (U32.v idx))) m borrows)
+                       (Seq.create 1 emp));
+     rewrite_equiv (value_vprops vp (Seq.create 1 (Seq.index s (U32.v idx))) m borrows) emp;
+     value_vprop_seq_upd_seq_and_repr h vp s m borrows (U32.v idx) i x c;
+     rewrite
+       (value_vprops vp (Seq.slice s 0 (U32.v idx)) m borrows
+          `star`
+        value_vprops vp (Seq.slice s (U32.v idx+1) (Seq.length s)) m borrows)
+       (value_vprops vp (Seq.slice (Seq.upd s (U32.v idx) (Some (i, x))) 0 (U32.v idx)) (Map.upd i (G.reveal c) m) borrows
+          `star`
+        value_vprops vp (Seq.slice (Seq.upd s (U32.v idx) (Some (i, x))) (U32.v idx+1) (Seq.length (Seq.upd s (U32.v idx) (Some (i, x))))) (Map.upd i (G.reveal c) m) borrows);
+
+     rewrite (vp i x c)
+             (vp i x (Some?.v (Map.sel i (Map.upd i (G.reveal c) m))));
+     SeqPerm.foldm_snoc_singleton vprop_monoid
+       (vp i x (Some?.v (Map.sel i (Map.upd i (G.reveal c) m))));
+     store_and_borrows_related bv s borrows;
+     assert (Seq.index
+               (value_vprops_seq vp (Seq.upd s (U32.v idx) (Some (i, x))) (Map.upd i (G.reveal c) m) borrows)
+               (U32.v idx) ==
+               vp i x (Some?.v (Map.sel i (Map.upd i (G.reveal c) m))));
+     assert (Seq.equal (value_vprops_seq vp (Seq.create 1 (Seq.index (Seq.upd s (U32.v idx) (Some (i, x))) (U32.v idx))) (Map.upd i (G.reveal c) m) borrows)
+                       (Seq.create 1 (vp i x (Some?.v (Map.sel i (Map.upd i (G.reveal c) m))))));
+     rewrite_equiv
+       (vp i x (Some?.v (Map.sel i (Map.upd i (G.reveal c) m))))
+       (value_vprops vp (Seq.create 1 (Seq.index (Seq.upd s (U32.v idx) (Some (i, x))) (U32.v idx))) (Map.upd i (G.reveal c) m) borrows);
+
+     value_vprops_split3 vp (Seq.upd s (U32.v idx) (Some (i, x))) (Map.upd i (G.reveal c) m) borrows (U32.v idx);
+     rewrite_equiv
+       (value_vprops vp (Seq.slice (Seq.upd s (U32.v idx) (Some (i, x))) 0 (U32.v idx)) (Map.upd i (G.reveal c) m) borrows
+          `star`
+        value_vprops vp (Seq.create 1 (Seq.index (Seq.upd s (U32.v idx) (Some (i, x))) (U32.v idx))) (Map.upd i (G.reveal c) m) borrows
+          `star`
+        value_vprops vp (Seq.slice (Seq.upd s (U32.v idx) (Some (i, x))) (U32.v idx+1) (Seq.length (Seq.upd s (U32.v idx) (Some (i, x))))) (Map.upd i (G.reveal c) m) borrows)
+       (value_vprops vp (Seq.upd s (U32.v idx) (Some (i, x))) (Map.upd i (G.reveal c) m) borrows);
+
+     intro_pure (pure_invariant a (Map.upd i (G.reveal c) m) borrows bv (Seq.upd s (U32.v idx) (Some (i, x))));
+
+     intro_exists (Seq.upd s (U32.v idx) (Some (i, x)))
+       (store_contents_pred_seq a (Map.upd i (G.reveal c) m) borrows bv);
+     intro_exists bv (store_contents_pred a (Map.upd i (G.reveal c) m) borrows);
+
+     assert (Map.equal (Map.remove i borrows) borrows);
+
+     rewrite (tperm a (Map.upd i (G.reveal c) m) borrows)
+             (put_post m borrows a i x c r)
+   | _ -> admit_ ());
+  return r
 
 let value_vprop_seq_rem_borrows
   (#k:eqtype)
